silveroak-opentitan/aes/Acorn/CipherEquivalenceNew.v
@@ -42,30 +42,44 @@ Require Import Cava.Acorn.Multistep.
 
 Require Import AesSpec.Cipher.
 Require Import AesSpec.CipherProperties.
-Require Import AesSpec.ExpandAllKeys.
-Require Import AesSpec.InterleavedCipher.
-Require Import AesSpec.InterleavedInverseCipher.
 Require Import AcornAes.CipherNewLoop.
 
 Existing Instance Combinational.CombinationalSemantics.
 
+Local Notation byte := (Vector.t bool 8).
+Local Notation state := (Vector.t (Vector.t byte 4) 4) (only parsing).
+Local Notation key := (Vector.t (Vector.t byte 4) 4) (only parsing).
+Local Notation round_index := (Vector.t bool 4) (only parsing).
+
+(* Helper definition to package the signals needed by the cipher loop *)
+Definition make_cipher_signals (Nr : nat) (is_decrypt : bool)
+           (init_key_input : list key)
+           (init_state_input : list state) :
+  list (bool * round_index * round_index * round_index * key * state) :=
+  (* assemble constant values + round index *)
+  let inner := map (fun i =>
+                      (is_decrypt, nat_to_bitvec_sized _ Nr,
+                       nat_to_bitvec_sized _ 0, nat_to_bitvec_sized _ i))
+                   (seq 0 (S Nr)) in
+  (* combine with initial key and initial state *)
+  combine (combine inner init_key_input) init_state_input.
+
+Lemma make_cipher_signals_length Nr is_decrypt init_key_input init_state_input :
+  length init_key_input = S Nr ->
+  length init_state_input = S Nr ->
+  length (make_cipher_signals
+            Nr is_decrypt init_key_input init_state_input) = S Nr.
+Proof. intros; cbv [make_cipher_signals]. length_hammer. Qed.
+Hint Rewrite @make_cipher_signals_length using solve [length_hammer] : push_length.
+
 Section WithSubroutines.
-  Local Notation byte := (Vector.t bool 8).
-  Local Notation state := (Vector.t (Vector.t byte 4) 4) (only parsing).
-  Local Notation key := (Vector.t (Vector.t byte 4) 4) (only parsing).
-  Local Notation round_index := (Vector.t bool 4) (only parsing).
-  Local Notation round_constant := byte (only parsing).
   Context (sub_bytes:     bool -> state -> ident state)
           (shift_rows:    bool -> state -> ident state)
           (mix_columns:   bool -> state -> ident state)
-          (add_round_key : key -> state -> ident state)
-          (key_expand : bool -> round_index -> key * round_constant ->
-                        ident (key * round_constant)).
+          (add_round_key : key -> state -> ident state).
   Context (sub_bytes_spec shift_rows_spec mix_columns_spec inv_sub_bytes_spec
                           inv_shift_rows_spec inv_mix_columns_spec : state -> state)
-          (add_round_key_spec : state -> key -> state)
-          (key_expand_spec inv_key_expand_spec :
-             nat -> key * round_constant -> key * round_constant).
+          (add_round_key_spec : state -> key -> state).
   Context
     (sub_bytes_correct : forall (is_decrypt : bool) (st : state),
         unIdent (sub_bytes is_decrypt st)
@@ -77,46 +91,25 @@ Section WithSubroutines.
         unIdent (mix_columns is_decrypt st)
         = if is_decrypt then inv_mix_columns_spec st else mix_columns_spec st)
     (add_round_key_correct :
-       forall k (st : state), unIdent (add_round_key k st) = add_round_key_spec st k)
-    (key_expand_correct :
-       forall (is_decrypt : bool) (round_i : round_index) (k : key) (rcon : round_constant),
-         unIdent (key_expand is_decrypt round_i (k,rcon))
-         = let spec := if is_decrypt then inv_key_expand_spec else key_expand_spec in
-           let i := N.to_nat (Bv2N round_i) in
-           (spec i (k, rcon))).
+       forall k (st : state), unIdent (add_round_key k st) = add_round_key_spec st k).
 
-  Let add_round_key_spec' : state -> key * round_constant -> state :=
-    (fun st k => add_round_key_spec st (fst k)).
-  Let inv_mix_columns_key_spec : key * round_constant -> key * round_constant :=
-    (fun '(k,rcon) => (inv_mix_columns_spec k, rcon)).
-  Let fwd_round_spec : key * round_constant * state -> nat -> key * round_constant * state :=
-    cipher_round_interleaved
-      add_round_key_spec' sub_bytes_spec shift_rows_spec mix_columns_spec
-      key_expand_spec.
-  Let inv_round_spec : key * round_constant * state -> nat -> key * round_constant * state :=
-    equivalent_inverse_cipher_round_interleaved
-      add_round_key_spec' inv_sub_bytes_spec inv_shift_rows_spec
-      inv_mix_columns_spec inv_key_expand_spec
-      inv_mix_columns_key_spec.
-  Let round_spec (is_decrypt : bool) (key_rcon_data : key * round_constant * state) (i : nat)
-    : key * round_constant * state :=
-    if is_decrypt then inv_round_spec key_rcon_data i else fwd_round_spec key_rcon_data i.
-  Let last_round_spec (is_decrypt : bool) (key_rcon_data : key * round_constant * state) (i : nat)
-    : key * round_constant * state :=
-    if is_decrypt
-    then
-      (inv_key_expand_spec i (fst key_rcon_data),
-       add_round_key_spec
-         (inv_shift_rows_spec (inv_sub_bytes_spec (snd key_rcon_data)))
-         (fst (fst key_rcon_data)))
-    else
-      (key_expand_spec i (fst key_rcon_data),
-       add_round_key_spec
-         (shift_rows_spec (sub_bytes_spec (snd key_rcon_data)))
-         (fst (fst key_rcon_data))).
+  (* Formula for each round based on index *)
+  Let round_spec (Nr : nat) (is_decrypt : bool) (k : key) (st : state) (i : nat) : state :=
+    if i =? 0
+    then add_round_key_spec st k
+    else if is_decrypt
+         then if i =? Nr
+              then add_round_key_spec (inv_shift_rows_spec (inv_sub_bytes_spec st)) k
+              else add_round_key_spec
+                     (inv_mix_columns_spec (inv_shift_rows_spec (inv_sub_bytes_spec st)))
+                     (inv_mix_columns_spec k)
+         else if i =? Nr
+              then add_round_key_spec (shift_rows_spec (sub_bytes_spec st)) k
+              else add_round_key_spec
+                     (mix_columns_spec (shift_rows_spec (sub_bytes_spec st))) k.
 
   Hint Rewrite sub_bytes_correct shift_rows_correct mix_columns_correct add_round_key_correct
-       key_expand_correct : to_spec.
+       : to_spec.
 
   Local Ltac simplify_step :=
     first [ destruct_pair_let
@@ -127,10 +120,8 @@ Section WithSubroutines.
           | progress cbn [fst snd map] ].
   Local Ltac simplify := repeat simplify_step.
 
-  (* key_expand_and_round is equivalent to interleaved cipher rounds *)
-  Lemma key_expand_and_round_equiv
-        (is_decrypt : bool)
-        (key_rcon_data : key * round_constant * state)
+  Lemma cipher_round_equiv
+        (is_decrypt : bool) (k : key) (data : state)
         add_round_key_in_sel round_key_sel
         (i Nr : nat) :
     Nr <> 0 -> i < 2 ^ 4 ->
@@ -141,34 +132,24 @@ Section WithSubroutines.
                      then if Nat.eqb i 0 then false
                           else if Nat.eqb i Nr then false else true
                      else false) ->
-    unIdent (key_expand_and_round
+    unIdent (cipher_round
                (key:=Vec (Vec (Vec Bit 8) 4) 4)
-               (round_constant:=Vec Bit 8)
                (state:=Vec (Vec (Vec Bit 8) 4) 4)
                (round_index:=Vec Bit 4)
-               sub_bytes shift_rows mix_columns add_round_key
-               (mix_columns true) key_expand
-               is_decrypt key_rcon_data add_round_key_in_sel round_key_sel
-               (nat_to_bitvec_sized _ i))
-    = if Nat.eqb i Nr
-      then last_round_spec is_decrypt key_rcon_data i
-      else round_spec is_decrypt key_rcon_data i.
+               sub_bytes shift_rows mix_columns add_round_key (mix_columns true)
+               is_decrypt k add_round_key_in_sel round_key_sel
+               (nat_to_bitvec_sized _ i) data)
+    = round_spec Nr is_decrypt k data i.
   Proof.
-    cbv zeta; intros. subst_lets. subst.
-    destruct key_rcon_data as [[round_key rcon] data].
-    cbv [key_expand_and_round cipher_round_interleaved mcompose
-                              equivalent_inverse_cipher_round_interleaved ].
-    simplify.
+    cbv zeta; intros. subst_lets. subst. destruct_products.
+    cbv [cipher_round mcompose]. simplify.
     repeat (destruct_one_match || destruct_one_match_hyp);
-      try Lia.lia; try congruence.
-    all:rewrite <-surjective_pairing.
-    all:reflexivity.
+      try Lia.lia; try congruence; reflexivity.
   Qed.
 
   Lemma cipher_step_equiv
         (Nr : nat) (is_decrypt is_first_round : bool)
-        (num_regular_rounds : round_index)
-        (key_rcon_data : key * round_constant * state)
+        (num_regular_rounds : round_index) (k : key) (data : state)
         (i : nat) :
     (* Nr must be at least two and small enough to fit in round_index size *)
     1 < Nr < 2 ^ 4 -> i <= Nr ->
@@ -177,32 +158,29 @@ Section WithSubroutines.
     unIdent
       (cipher_step
          (key:=Vec (Vec (Vec Bit 8) 4) 4)
-         (round_constant:=Vec Bit 8)
          (state:=Vec (Vec (Vec Bit 8) 4) 4)
          (round_index:=Vec Bit 4)
          sub_bytes shift_rows mix_columns add_round_key (mix_columns true)
-         key_expand is_decrypt is_first_round num_regular_rounds
-         key_rcon_data (nat_to_bitvec_sized _ i))
-    = if i =? Nr
-      then last_round_spec is_decrypt key_rcon_data i
-      else round_spec is_decrypt key_rcon_data i.
+         is_decrypt is_first_round num_regular_rounds
+         k (nat_to_bitvec_sized _ i) data)
+    = round_spec Nr is_decrypt k data i.
   Proof.
     cbv zeta; intro Hall_keys; intros. subst.
-    cbv [cipher_step]. simplify.
+    cbv [cipher_step]. simplify. destruct_products.
 
     (* simplify boolean comparisons *)
     cbn [nor2 and2 CombinationalSemantics].
     simplify.
 
-    apply key_expand_and_round_equiv with (Nr:=Nr);
+    apply cipher_round_equiv with (Nr:=Nr);
       try Lia.lia; repeat destruct_one_match;
         boolsimpl; reflexivity.
   Qed.
 
   Lemma cipher_loop_step
         (Nr : nat) (num_regular_rounds round0 : round_index)
-        (is_decrypt : bool) (init_cipher_state : key * round_constant * state)
-        (round_i : round_index) (i : nat) :
+        (is_decrypt : bool) (init_key : key) (init_state : state)
+        (round_key : key) (round_i : round_index) (i : nat) :
     (* Nr must be at least two and small enough to fit in round_index size *)
     1 < Nr < 2 ^ 4 ->
     0 <= i <= Nr ->
@@ -211,84 +189,69 @@ Section WithSubroutines.
     round0 = nat_to_bitvec_sized _ 0 ->
     let loop := cipher_loop
                   (key:=Vec (Vec (Vec Bit 8) 4) 4)
-                  (round_constant:=Vec Bit 8)
                   (state:=Vec (Vec (Vec Bit 8) 4) 4)
                   (round_index:=Vec Bit 4)
-                  sub_bytes shift_rows mix_columns add_round_key (mix_columns true)
-                  key_expand in
-    forall current_cipher_state : circuit_state loop,
-      let key := snd current_cipher_state in
-      let rcon := snd (fst current_cipher_state) in
-      let state := snd (fst (fst current_cipher_state)) in
+                  sub_bytes shift_rows mix_columns add_round_key (mix_columns true) in
+    forall current_state : circuit_state loop,
       unIdent
-        (interp loop current_cipher_state
+        (interp loop current_state
                 (is_decrypt, num_regular_rounds, round0, round_i,
-                 init_cipher_state))
-      = let st := if i =? 0 then init_cipher_state else (key,rcon,state) in
-        let out := (if i =? Nr
-                    then last_round_spec is_decrypt st i
-                    else round_spec is_decrypt st i) in
-        (out, (tt, snd out, snd (fst out), fst (fst out))).
+                 init_key, init_state, round_key))
+      = let st := if i =? 0 then init_state else snd (current_state) in
+        let st' := round_spec Nr is_decrypt round_key st i in
+        (st', (tt, st')).
   Proof.
     cbv zeta; intros.
     subst round0 num_regular_rounds round_i.
     cbv [cipher_loop Loop] in *. cbn [interp circuit_state] in *.
-    destruct_products. repeat destruct_pair_let. cbn [fst snd].
-    simpl_ident. rewrite !eqb_nat_to_bitvec_sized by Lia.lia.
+    destruct_products. simplify.
     rewrite cipher_step_equiv with (Nr:=Nr)
       by (try Lia.lia; destruct i; reflexivity).
-    (* too many pair-lets to simplify them all straightaway; expose pairs first *)
-    destruct_inner_pair_let; cbn [unIdent].
-    destruct_inner_pair_let; cbn [unIdent].
     simplify.
     repeat destruct_one_match; cbn [fst snd].
-    all:rewrite <-!surjective_pairing.
     all:try Lia.lia.
     all:try reflexivity.
     all:exfalso; congruence.
   Qed.
 
-  (* Model the expected trace of the cipher loop using the interleaved cipher
-     definition *)
+  (* Model the expected trace of the cipher loop *)
   Definition cipher_trace_with_keys
-             (Nr : nat) (is_decrypt : bool) (first_key : key) (init_rcon : round_constant)
-             (input : state) : list (key * round_constant * state) :=
+             (Nr : nat) (is_decrypt : bool)
+             (init_state : state) (round_keys : list key) : list state :=
     (* Run all rounds except the last *)
     let '(acc, state) :=
         fold_left_accumulate
-          (fun st i =>
-             if i =? Nr
-             then last_round_spec is_decrypt st i
-             else round_spec is_decrypt st i)
-          (List.seq 0 (S Nr)) (first_key, init_rcon, input) in
+          (fun st '(i,k) =>
+             round_spec Nr is_decrypt k st i)
+          (combine (List.seq 0 (S Nr)) round_keys)
+          init_state in
     tl acc.
 
   Lemma cipher_loop_equiv
         (Nr : nat) (is_decrypt : bool)
-        (init_rcon : round_constant) (init_key : key) (init_state : state)
-        (cipher_input : list _) init_cipher_state_ignored :
+        init_key_ignored
+        (init_state : state) init_state_ignored
+        (round_keys : list key) (cipher_input : list _) :
     (* Nr must be at least two and small enough to fit in round_index size *)
     1 < Nr < 2 ^ 4 ->
-    let init_cipher_state := (init_key, init_rcon, init_state) in
-    length init_cipher_state_ignored = Nr ->
-    cipher_input = combine
-                     (map
-                        (fun i =>
-                           (is_decrypt, nat_to_bitvec_sized _ Nr,
-                            nat_to_bitvec_sized _ 0, nat_to_bitvec_sized _ i))
-                        (seq 0 (S Nr)))
-                     (init_cipher_state :: init_cipher_state_ignored) ->
+    length init_key_ignored = S Nr ->
+    length init_state_ignored = Nr ->
+    length round_keys = S Nr ->
+    cipher_input = make_cipher_signals
+                     Nr is_decrypt init_key_ignored
+                     (init_state :: init_state_ignored) ->
     let loop := cipher_loop
                   (key:=Vec (Vec (Vec Bit 8) 4) 4)
-                  (round_constant:=Vec Bit 8)
                   (state:=Vec (Vec (Vec Bit 8) 4) 4)
                   (round_index:=Vec Bit 4)
-                  sub_bytes shift_rows mix_columns add_round_key (mix_columns true)
-                  key_expand in
-    multistep loop cipher_input
-    = cipher_trace_with_keys Nr is_decrypt init_key init_rcon init_state.
+                  sub_bytes shift_rows mix_columns add_round_key (mix_columns true) in
+    multistep loop (combine cipher_input round_keys)
+    = cipher_trace_with_keys Nr is_decrypt init_state round_keys.
   Proof.
     cbv zeta; intros. subst cipher_input.
+    cbv [make_cipher_signals] in *.
+    destruct round_keys; cbn [length] in *; [ length_hammer | ].
+    destruct init_key_ignored; cbn [length] in *; [ length_hammer | ].
     cbv [multistep cipher_trace_with_keys].
     cbn [seq map combine].
     rewrite fold_left_accumulate_cons_full.
@@ -304,24 +267,29 @@ Section WithSubroutines.
     (* Use loop invariant *)
     rewrite fold_left_accumulate_to_seq
       with (default := (defaultCombValue _, defaultCombValue _, defaultCombValue _,
-                        defaultCombValue _, (defaultCombValue _, defaultCombValue _,
-                                             defaultCombValue _))).
+                        defaultCombValue _, defaultCombValue _, defaultCombValue _,
+                        defaultCombValue _)).
+    rewrite fold_left_accumulate_to_seq
+      with (default:=(0,defaultCombValue (Vec (Vec (Vec Bit 8) 4) 4))).
     autorewrite with push_length natsimpl.
-    rewrite <-seq_shift, fold_left_accumulate_map.
     factor_out_loops.
     eapply fold_left_accumulate_double_invariant_seq
-      with (I:=fun i st1 st2 => (st1 = (st2, (tt, snd st2, snd (fst st2), fst (fst st2))))).
+      with (I:=fun i st1 st2 => (st1 = (st2, (tt, st2)))).
     { (* invariant holds at start *)
       reflexivity. }
     { (* invariant holds through body *)
       intros i x y; intros; subst x. cbn [fst snd].
-      rewrite map_map. autorewrite with push_nth.
+      rewrite <-!seq_shift, !map_map.
+      rewrite !combine_map_l.
+      erewrite map_nth_inbounds with (d2:=(0,init_state,init_state,init_state)) by length_hammer.
+      erewrite map_nth_inbounds with (d2:=(0,init_state)) by length_hammer.
+      cbn [combType] in *.
+      autorewrite with push_nth natsimpl. cbn [fst snd].
       erewrite cipher_loop_step with (Nr:=Nr) (i:=S i)
         by (reflexivity || Lia.lia).
-      cbn zeta delta [fst snd]. repeat destruct_pair_let.
+      cbn [fst snd]. repeat destruct_pair_let.
       cbn [fst snd]. change (S i =? 0) with false. cbn match.
-      destruct_products. cbn [fst snd].
-      destr (i =? Nr); reflexivity. }
+      destruct_products. reflexivity. }
     { (* invariant implies postcondition *)
       intros *. intros Heq Hnth; intros.
       rewrite Heq in *. cbn [fst snd].
@@ -348,159 +316,104 @@ Section WithSubroutines.
       reflexivity. }
   Qed.
 
+  Lemma fold_round_spec_equiv (Nr : nat) (is_decrypt : bool)
+        init_key init_state middle_keys last_key :
+    0 < Nr ->
+    length middle_keys = Nr - 1 ->
+    fold_left (fun (st : t (t byte 4) 4) '(i, k) => round_spec Nr is_decrypt k st i)
+              (combine (seq 1 Nr) (middle_keys ++ [last_key]))
+              (round_spec Nr is_decrypt init_key init_state 0) =
+    if is_decrypt
+    then
+      Cipher.equivalent_inverse_cipher
+        _ _ add_round_key_spec inv_sub_bytes_spec inv_shift_rows_spec
+        inv_mix_columns_spec init_key last_key
+        (map inv_mix_columns_spec middle_keys) init_state
+    else
+      Cipher.cipher _ _ add_round_key_spec sub_bytes_spec shift_rows_spec
+                    mix_columns_spec init_key last_key middle_keys init_state.
+  Proof.
+    intros. rewrite <-seq_shift, combine_map_l.
+    rewrite fold_left_map. destruct Nr; [ Lia.lia | ].
+    autorewrite with pull_snoc.
+    rewrite combine_append by length_hammer.
+    cbn [combine]. autorewrite with pull_snoc natsimpl.
+    cbn [fst snd].
+    cbv [equivalent_inverse_cipher Cipher.cipher].
+    rewrite fold_left_to_seq with (default:=(0,init_key)).
+    rewrite !fold_left_to_seq with (default:=init_key).
+    autorewrite with push_length natsimpl.
+    replace (length middle_keys) with Nr by Lia.lia.
+    destruct is_decrypt.
+    { cbv [round_spec]. repeat destruct_one_match; try Lia.lia; [ ].
+      factor_out_loops.
+      eapply fold_left_double_invariant_seq with
+          (I:=fun _ st1 st2 => st1 = st2);
+        [ reflexivity | | congruence ].
+      intros; subst.
+      autorewrite with push_nth natsimpl. cbn [fst snd].
+      rewrite map_nth_inbounds with (d2:=init_key) by length_hammer.
+      repeat destruct_one_match; try Lia.lia. reflexivity. }
+    { cbv [round_spec]. repeat destruct_one_match; try Lia.lia; [ ].
+      factor_out_loops.
+      eapply fold_left_double_invariant_seq with
+          (I:=fun _ st1 st2 => st1 = st2);
+        [ reflexivity | | congruence ].
+      intros; subst.
+      autorewrite with push_nth natsimpl. cbn [fst snd].
+      repeat destruct_one_match; try Lia.lia. reflexivity. }
+  Qed.
+
   Lemma cipher_equiv
-        (Nr : nat)
-        init_cipher_state_ignored
-        (init_rcon : round_constant) (init_key : key) (init_state : state)
+        (key_expand : Circuit _ _)
+        (Nr : nat) init_key_input init_state_ignored
+        (is_decrypt : bool)
+        (init_key : key) (init_state : state)
         (last_key : key) (middle_keys : list key)
-        (cipher_input : list _) :
-    (* precomputed keys match key expansion *)
-    let all_keys_and_rcons := all_keys key_expand_spec Nr (init_key, init_rcon) in
-    let all_keys := List.map fst all_keys_and_rcons in
-    all_keys = (init_key :: middle_keys ++ [last_key])%list ->
-    (* Nr must be at least two and small enough to fit in round_index size *)
+        (cipher_input : list _) :(* Nr must be at least two and small enough to fit in round_index size *)
     1 < Nr < 2 ^ 4 ->
-    let init_cipher_state := (init_key, init_rcon, init_state) in
-    length init_cipher_state_ignored = Nr ->
-    cipher_input = combine
-                     (map
-                        (fun i =>
-                           (false, nat_to_bitvec_sized _ Nr,
-                            nat_to_bitvec_sized _ 0, nat_to_bitvec_sized _ i))
-                        (seq 0 (S Nr)))
-                     (init_cipher_state :: init_cipher_state_ignored) ->
+    length init_key_input = S Nr ->
+    length init_state_ignored = Nr ->
+    length middle_keys = Nr - 1 ->
+    cipher_input = make_cipher_signals Nr is_decrypt init_key_input
+                                       (init_state :: init_state_ignored) ->
+    (* precomputed keys match key expansion *)
+    multistep key_expand cipher_input = init_key :: middle_keys ++ [last_key] ->
     let cipher := cipher
                     (key:=Vec (Vec (Vec Bit 8) 4) 4)
-                    (round_constant:=Vec Bit 8)
                     (state:=Vec (Vec (Vec Bit 8) 4) 4)
                     (round_index:=Vec Bit 4)
                     sub_bytes shift_rows mix_columns add_round_key (mix_columns true)
                     key_expand in
     forall d,
       nth Nr (multistep cipher cipher_input) d
-      = AesSpec.Cipher.cipher
-          _ _ add_round_key_spec sub_bytes_spec shift_rows_spec mix_columns_spec
-          init_key last_key middle_keys init_state.
+      = if is_decrypt
+        then
+          Cipher.equivalent_inverse_cipher
+            _ _ add_round_key_spec inv_sub_bytes_spec inv_shift_rows_spec
+            inv_mix_columns_spec init_key last_key
+            (map inv_mix_columns_spec middle_keys) init_state
+        else
+          Cipher.cipher
+            _ _ add_round_key_spec sub_bytes_spec shift_rows_spec
+            mix_columns_spec init_key last_key middle_keys init_state.
   Proof.
-    cbv zeta; intro Hall_keys; intros. subst cipher_input.
-    cbv [cipher]. rewrite multistep_compose, multistep_comb.
-    erewrite map_ext with (g:=snd) by (intros; destruct_products; reflexivity).
-    erewrite cipher_loop_equiv with (Nr:=Nr)
-      by (eassumption||reflexivity).
+    cbv zeta; intros. subst cipher_input.
+    cbv [cipher]. autorewrite with push_multistep.
+    rewrite !map_map.
+    rewrite !ListUtils.map_id_ext by reflexivity.
+    erewrite cipher_loop_equiv with (Nr:=Nr) (init_state_ignored:=init_state_ignored)
+      by length_hammer.
+    match goal with Hkexp : multistep key_expand _ = _ |- _ =>
+                    cbv [combType Bvector.Bvector] in Hkexp |- *;
+                      rewrite Hkexp; clear Hkexp end.
     cbv [cipher_trace_with_keys]. simplify.
 
-    (* simplify selection of last element *)
-    erewrite map_nth_inbounds
-      with (d2:=defaultCombValue
-                  (Pair (Pair (Vec (Vec (Vec Bit 8) 4) 4) (Vec Bit 8))
-                        (Vec (Vec (Vec Bit 8) 4) 4)))
-      by length_hammer.
-    autorewrite with push_nth. rewrite nth_tl, nth_last by length_hammer.
-    rewrite fold_left_accumulate_last.
+    cbn [seq combine]. rewrite fold_left_accumulate_cons.
+    cbn [tl]. rewrite nth_fold_left_accumulate by length_hammer.
+    rewrite !firstn_all2 by length_hammer.
 
-    (* Get all states from key expansion *)
-    map_inversion Hall_keys; subst.
-    match goal with H : @eq (list (_ * _)) _ (_ :: _ ++ [_])%list |- _ =>
-                    rename H into Hall_keys end.
-
-    (* representation change; use full key-expansion state (key * round_constant) *)
-    erewrite cipher_change_key_rep with (projkey:=@fst key round_constant)
-      by (reflexivity || eauto).
-
-    erewrite <-cipher_interleaved_equiv by eassumption.
-    cbv [cipher_interleaved]. repeat destruct_pair_let.
-
-    (* process last round on LHS *)
-    autorewrite with pull_snoc.
-    destruct_one_match; try Lia.lia; [ ].
-
-    (* remove the last-round case from loop body *)
-    erewrite ListUtils.fold_left_ext_In with (f:= fun _ _ => if _ =? _ then _ else _)
-      by (intros *; rewrite in_seq; intros; repeat destruct_one_match; try Lia.lia;
-          reflexivity).
-
-    reflexivity.
-  Qed.
-
-  Lemma inv_mix_columns_key_spec_map keys :
-    map fst (map inv_mix_columns_key_spec keys) = map inv_mix_columns_spec (map fst keys).
-  Proof.
-    rewrite !map_map; apply map_ext.
-    intros; subst_lets. cbv beta.
-    repeat destruct_pair_let; reflexivity.
-  Qed.
-
-  Lemma inverse_cipher_equiv
-        (Nr : nat) init_cipher_state_ignored
-        (init_rcon : round_constant) (init_key : key) (init_state : state)
-        (last_key : key) (middle_keys : list key)
-        (cipher_input : list _) :
-    (* precomputed keys match key expansion *)
-    let all_keys_and_rcons := all_keys inv_key_expand_spec Nr (init_key, init_rcon) in
-    let all_keys := List.map fst all_keys_and_rcons in
-    all_keys = (init_key :: middle_keys ++ [last_key])%list ->
-    (* Nr must be at least two and small enough to fit in round_index size *)
-    1 < Nr < 2 ^ 4 ->
-    let init_cipher_state := (init_key, init_rcon, init_state) in
-    length init_cipher_state_ignored = Nr ->
-    cipher_input = combine
-                     (map
-                        (fun i =>
-                           (true, nat_to_bitvec_sized _ Nr,
-                            nat_to_bitvec_sized _ 0, nat_to_bitvec_sized _ i))
-                        (seq 0 (S Nr)))
-                     (init_cipher_state :: init_cipher_state_ignored) ->
-    let cipher := cipher
-                    (key:=Vec (Vec (Vec Bit 8) 4) 4)
-                    (round_constant:=Vec Bit 8)
-                    (state:=Vec (Vec (Vec Bit 8) 4) 4)
-                    (round_index:=Vec Bit 4)
-                    sub_bytes shift_rows mix_columns add_round_key (mix_columns true)
-                    key_expand in
-    forall d,
-      nth Nr (multistep cipher cipher_input) d
-      = Cipher.equivalent_inverse_cipher
-         _ _ add_round_key_spec inv_sub_bytes_spec inv_shift_rows_spec inv_mix_columns_spec
-         init_key last_key (map inv_mix_columns_spec middle_keys) init_state.
-  Proof.
-    cbv zeta; intro Hall_keys; intros. subst cipher_input.
-    cbv [cipher]. rewrite multistep_compose, multistep_comb.
-    erewrite map_ext with (g:=snd) by (intros; destruct_products; reflexivity).
-    erewrite cipher_loop_equiv with (Nr:=Nr) by (eassumption||reflexivity).
-    cbv [cipher_trace_with_keys]. simplify.
-
-    (* simplify selection of last element *)
-    erewrite map_nth_inbounds
-      with (d2:=defaultCombValue
-                  (Pair (Pair (Vec (Vec (Vec Bit 8) 4) 4) (Vec Bit 8))
-                        (Vec (Vec (Vec Bit 8) 4) 4)))
-      by length_hammer.
-    autorewrite with push_nth. rewrite nth_tl, nth_last by length_hammer.
-    rewrite fold_left_accumulate_last.
-
-    (* Get all states from key expansion *)
-    map_inversion Hall_keys; subst.
-    match goal with H : @eq (list (_ * _)) _ (_ :: _ ++ [_])%list |- _ =>
-                    rename H into Hall_keys end.
-
-    (* representation change; use full key-expansion state (key * round_constant) *)
-    erewrite equivalent_inverse_cipher_change_key_rep
-      with (projkey:=@fst key round_constant)
-           (middle_keys_alt:=List.map inv_mix_columns_key_spec _)
-      by (reflexivity || apply inv_mix_columns_key_spec_map).
-
-    erewrite <-equivalent_inverse_cipher_interleaved_equiv by eassumption.
-    cbv [equivalent_inverse_cipher_interleaved]. repeat destruct_pair_let.
-
-    (* process last round on LHS *)
-    autorewrite with pull_snoc.
-    destruct_one_match; try Lia.lia; [ ].
-
-    (* remove the last-round case from loop body *)
-    erewrite ListUtils.fold_left_ext_In with (f:= fun _ _ => if _ =? _ then _ else _)
-      by (intros *; rewrite in_seq; intros; repeat destruct_one_match; try Lia.lia;
-          reflexivity).
-
+    erewrite <-fold_round_spec_equiv with (Nr:=Nr) by length_hammer.
     reflexivity.
   Qed.
 End WithSubroutines.
